Restructure initiator with higher-level tagging and list primitives

lib.v
@@ -8,31 +8,103 @@ Definition flipb {T S} (b : bool) (f : T → T → S) x y :=
   f (if b then x else y) (if b then y else x).
 
 Class Repr A := repr : A -> val.
+Arguments repr / .
 
 Instance repr_Z : Repr Z := λ x, #x.
+Arguments repr_Z / .
 
 Instance repr_option `{Repr A} : Repr (option A) := λ x,
   match x with
   | Some x => SOMEV (repr x)
   | None => NONEV
   end.
+Arguments repr_option {A} {_} !_.
 
-Instance repr_list `{Repr A} : Repr (list A) :=
-  fold_right (fun x v => (repr x, v)%V) #0.
+Definition repr_list_aux `{Repr A} :
+  seal (foldr (fun x v => SOMEV (repr x, v)%V) NONEV).
+  by eexists.
+Qed.
+Instance repr_list `{Repr A} : Repr (list A) := unseal repr_list_aux.
+Arguments repr_list {A} {_} _ : simpl never.
+
+Lemma repr_list_eq `{Repr A} :
+  repr_list = foldr (fun x v => SOMEV (repr x, v)%V) NONEV.
+Proof. exact: seal_eq. Qed.
+
+Existing Instance repr_list.
 
 Definition get_list : val := rec: "loop" "l" "n" :=
-  if: "l" = #0 then NONE
-  else if: "n" = #0 then SOME (Fst "l")
-  else "loop" (Snd "l") ("n" - #1).
+  match: "l" with NONE => NONE
+  | SOME "p" =>
+    if: "n" = #0 then SOME (Fst "p")
+    else "loop" (Snd "p") ("n" - #1)
+  end.
 
-Lemma twp_get_list `{!Repr A, !heapG Σ} (l : list A) (n : nat) :
-  ⊢ WP get_list (repr l) #n
-       [{v, ⌜v = repr (nth_error l n)⌝}].
+Notation "l !! n" := (get_list l n) : expr_scope.
+
+Definition NILV : val := NONEV.
+Definition CONSV hd tl : val := SOMEV (hd, tl).
+Notation "hd :: tl" := (CONSV hd%V tl%V) : val_scope.
+Notation "[ ]" := (NILV) : val_scope.
+Notation "[ x ]" := (CONSV x%V NILV) : val_scope.
+Notation "[ x ; y ; .. ; z ]" :=
+  (CONSV x%V (CONSV y%V .. (CONSV z%V NILV) ..)) : val_scope.
+
+Definition NIL : expr := NONE.
+Definition CONS : val := λ: "hd" "tl", SOME ("hd", "tl").
+Notation "hd :: tl" := (CONS hd%E tl%E) : expr_scope.
+Notation "[ ]" := (NIL) : expr_scope.
+Notation "[ x ]" := (CONS x%V NIL) : expr_scope.
+Notation "[ x ; y ; .. ; z ]" :=
+  (CONS x%E (CONS y%E .. (CONS z%E NIL) ..)) : expr_scope.
+
+Section ListLemmas.
+
+Context `{!Repr A, !heapG Σ}.
+
+Lemma twp_get_list E (l : list A) (n : nat) Ψ :
+  Ψ (repr (l !! n)) -∗
+  WP repr l !! #n @ E [{ Ψ }].
 Proof.
-rewrite /repr; elim: n l=> [|n IH] [|x l] /=; wp_rec; wp_pures; eauto.
+rewrite /= repr_list_eq.
+elim: n l Ψ => [|n IH] [|x l] /= Ψ; iIntros "post";
+wp_rec; wp_pures; eauto.
 rewrite (_ : (S n - 1)%Z = n); try lia.
 by iApply IH.
 Qed.
 
-Instance prod_repr `{Repr A, Repr B} : Repr (A * B) :=
+Lemma wp_get_list E (l : list A) (n : nat) Ψ :
+  Ψ (repr (l !! n)) -∗
+  WP repr l !! #n @ E {{ Ψ }}.
+Proof. by iIntros "?"; iApply twp_wp; iApply twp_get_list. Qed.
+
+Lemma twp_nil E Ψ :
+  Ψ (repr (@nil A)) -∗
+  WP []%V @ E [{ Ψ }].
+Proof.
+rewrite /NILV /= repr_list_eq; iIntros "?"; wp_pures.
+by iApply twp_value. (* FIXME *)
+Qed.
+
+Lemma wp_nil E Ψ :
+  Ψ (repr (@nil A)) -∗
+  WP []%V @ E {{ Ψ }}.
+Proof. by iIntros "?"; iApply twp_wp; iApply twp_nil. Qed.
+
+Lemma twp_cons E x xs Ψ :
+  Ψ (repr (x :: xs)) -∗
+  WP repr x :: repr xs @ E [{ Ψ }].
+Proof.
+rewrite /= repr_list_eq; iIntros "post"; by rewrite /CONS; wp_pures.
+Qed.
+
+Lemma wp_cons E x xs Ψ :
+  Ψ (repr (x :: xs)) -∗
+  WP repr x :: repr xs @ E {{ Ψ }}.
+Proof. by iIntros "?"; iApply twp_wp; iApply twp_cons. Qed.
+
+End ListLemmas.
+
+Instance repr_prod `{Repr A, Repr B} : Repr (A * B) :=
   λ p, (repr p.1, repr p.2)%V.
+Arguments repr_prod {_ _ _ _} !_.
